C1_Schreier_vector.v
@@ -8,16 +8,16 @@ Section Vector.
 Definition vector := fmap perm.
 
 (* Add all numbers reachable from i. *)
-Fixpoint extend (i : positive) (h : perm)
+Fixpoint extend (i : positive) (π : perm)
   (gen : list perm) (V : vector)
   (new : list positive) :=
   match gen with
   | [] => (V, new)
-  | g :: gen' =>
-    let j := g⋅i in
+  | σ :: gen' =>
+    let j := σ⋅i in
     match lookup V j with
-    | Some _ => extend i h gen' V new
-    | None => extend i h gen' (insert V j (g ∘ h)) (j :: new)
+    | Some _ => extend i π gen' V new
+    | None => extend i π gen' (insert V j (σ ∘ π)) (j :: new)
     end
   end.
 
@@ -31,8 +31,8 @@ Fixpoint extend_loop (V : vector) (try new : list positive) :=
   | i :: try' =>
     match lookup V i with
     | None => extend_loop V try' new
-    | Some h =>
-      match extend i h gen V new with
+    | Some π =>
+      match extend i π gen V new with
       | (V', new') => extend_loop V' try' new'
       end
     end
@@ -69,6 +69,37 @@ Definition generators (V : vector) : list perm :=
 Theorems
 *)
 
+Ltac replace_fst x y E := replace x with (fst (x, y)) by easy; rewrite <-E.
+Ltac replace_snd x y E := replace y with (snd (x, y)) by easy; rewrite <-E.
+
+Section Generic.
+
+Open Scope nat.
+
+Variable P : vector -> Prop.
+Hypothesis prop_extend_loop :
+  ∀V try new, P V -> P (fst (extend_loop V try new)).
+
+Lemma prop_loop V try n :
+  P V -> P (loop V try n).
+Proof.
+revert V try; simple_ind n.
+destruct (extend_loop _) as [V' new] eqn:E.
+replace_fst V' new E; destruct new; [|apply IHn].
+all: apply prop_extend_loop, H.
+Qed.
+
+Lemma prop_loop_le V try m n :
+  P (loop V try m) -> m <= n -> P (loop V try n).
+Proof.
+revert V try n; induction m; simpl; intros.
+apply prop_loop, H. destruct n; [easy|simpl].
+destruct (extend_loop _) as [V' new] eqn:E.
+destruct new; [easy|]. apply IHm. easy. apply le_S_n, H0.
+Qed.
+
+End Generic.
+
 Section Soundness.
 
 (* The orbit permutations are valid. *)
@@ -78,9 +109,9 @@ Definition Sound (V : vector) := ∀i,
   | None => True
   end.
 
-Lemma sound_extend h gen' V new :
-  Generates gen h -> gen' ⊆ gen ->
-  Sound V -> Sound (fst (extend h⋅k h gen' V new)).
+Lemma sound_extend π gen' V new :
+  Generates gen π -> gen' ⊆ gen ->
+  Sound V -> Sound (fst (extend π⋅k π gen' V new)).
 Proof.
 revert V new; simple_ind gen'.
 apply incl_cons_inv in H0 as [].
@@ -94,26 +125,17 @@ Lemma sound_extend_loop V try new :
   Sound V -> Sound (fst (extend_loop V try new)).
 Proof.
 revert V new; simple_ind try.
-destruct (lookup V a) eqn:E. destruct (extend _) as [V' new'] eqn:E'.
-replace V' with (fst (extend a p gen V new)) by (rewrite E'; easy).
-all: apply IHtry. assert(Ha := H a); rewrite E in Ha; destruct Ha; subst.
-apply sound_extend; easy. easy.
-Qed.
-
-Lemma sound_loop V try n :
-  Sound V -> Sound (loop V try n).
-Proof.
-revert V try; simple_ind n.
-destruct (extend_loop _) as [V' new] eqn:E.
-replace V' with (fst (extend_loop V try [])) by (rewrite E; easy).
-destruct new. apply sound_extend_loop, H.
-apply IHn, sound_extend_loop, H.
+destruct (lookup V a) eqn:E.
+destruct (extend _) as [V' new'] eqn:E'.
+replace_fst V' new' E'. all: apply IHtry; try easy.
+assert(Ha := H a); rewrite E in Ha; destruct Ha; subst.
+apply sound_extend; easy.
 Qed.
 
 Theorem sound_build bound :
   Sound (build bound).
 Proof.
-apply sound_loop.
+unfold build; apply prop_loop. apply sound_extend_loop.
 intros i. rewrite lookup_insert; simpl.
 destruct (k =? i) eqn:E. convert_bool; subst.
 split. exists []; simpl; easy. easy. easy.
@@ -125,37 +147,94 @@ Section Completeness.
 
 Local Open Scope nat.
 
+(* The vector contains the full orbit. *)
+Definition Complete (V : vector) := ∀π, Generates gen π -> Defined V π⋅k.
+
 (* The vector and the new points are an intermediary result. *)
-Definition Intermediary (V : vector) new := Forall (λ i, Defined V i) new /\
+Definition Intermediate (V : vector) new :=
+  Forall (λ i, Defined V i) new /\
   ∀i, Defined V i -> In i new \/ ∀σ, In σ gen -> Defined V σ⋅i.
 
-(* The vector contains the full orbit. *)
-Definition Complete (V : vector) :=
-  ∀π, Generates gen π -> Defined V π⋅k.
+Lemma defined_extend i j π gen' V new :
+  Defined V i -> gen' ⊆ gen -> Defined (fst (extend j π gen' V new)) i.
+Proof.
+revert V new; simple_ind gen'. apply incl_cons_inv in H0.
+destruct (lookup V a⋅j) eqn:E; apply IHgen'; try easy.
+apply defined_before_insert, H.
+Qed.
 
 Lemma defined_extend_loop V try new i :
   Defined V i -> Defined (fst (extend_loop V try new)) i.
 Proof.
-Admitted.
+revert V new; simple_ind try.
+destruct (lookup V a) eqn:E.
+destruct (extend _) as [V' new'] eqn:E'.
+replace_fst V' new' E'. all: apply IHtry; try easy.
+apply defined_extend; easy.
+Qed.
 
-Lemma defined_loop V try m n i :
-  Defined (loop V try m) i -> m <= n -> Defined (loop V try n) i.
+Lemma not_new_extend i j π gen' V new :
+  Defined V i -> ¬In i new -> ¬In i (snd (extend j π gen' V new)).
 Proof.
-Admitted.
+revert V new; simple_ind gen'.
+destruct (lookup V a⋅j) eqn:E; apply IHgen'; try easy.
+apply defined_before_insert, H. intros []; [subst|easy].
+rewrite E in H; easy.
+Qed.
 
-Lemma intermediary_extend_loop V try new V' try' :
+Lemma not_new_extend_loop V try new i :
+  Defined V i -> ¬In i new -> ¬In i (snd (extend_loop V try new)).
+Proof.
+revert V new; simple_ind try.
+destruct (lookup V a) eqn:E.
+destruct (extend _) as [V' new'] eqn:E'.
+all: apply IHtry; try easy.
+replace_fst V' new' E'; apply defined_extend; easy.
+replace_snd V' new' E'; apply not_new_extend; easy.
+Qed.
+
+Lemma intermediate_extend try i π gen' V new V' new' :
+  extend i π gen' V new = (V', new') ->
+  gen' ⊆ gen -> (∀σ, In σ gen -> ¬In σ gen' -> Defined V σ⋅i) ->
+  Intermediate V (i :: try ++ new) -> Intermediate V' (try ++ new').
+Proof.
+revert V new; induction gen'; simpl; intros.
+- inv H; destruct H2. split. inv H. intros.
+  apply H2 in H3 as []. inv H3.
+  right; intros; apply H1; easy.
+  left; easy. right; easy.
+- apply incl_cons_inv in H0.
+  destruct (lookup _) eqn:E; eapply IHgen' in H; try easy; intros.
+  + destruct (ffun_eq_dec a σ); subst. rewrite E; easy.
+    apply H1. easy. intros []; easy.
+  + destruct (ffun_eq_dec a σ); subst. rewrite lookup_insert_eq; easy.
+    apply defined_before_insert, H1. easy. intros []; easy.
+  + destruct H2. rewrite app_comm_cons in H2; apply Forall_app in H2. split.
+    * apply Forall_app with (l1:=i :: try); split.
+      2: apply Forall_cons. 2: rewrite lookup_insert_eq; easy.
+      all: eapply Forall_impl; [|apply H2].
+      all: intros; apply defined_before_insert; easy.
+    * intros. rewrite lookup_insert in H4.
+      destruct (_ =? _)%positive eqn:E'; convert_bool; subst.
+      left; auto with datatypes. apply H3 in H4 as [].
+      left; rewrite app_comm_cons; apply in_app_comm, in_cons, in_app_comm, H4.
+      right; intros; apply defined_before_insert, H4, H5.
+Qed.
+
+Lemma intermediate_extend_loop V try new V' try' :
   extend_loop V try new = (V', try') ->
-  Intermediary V try -> Intermediary V' try'.
+  Intermediate V (try ++ new) -> Intermediate V' try'.
 Proof.
-Admitted.
+revert V new; induction try; simpl; intros. inv H.
+assert(Defined V a) by (destruct H0; inv H0).
+destruct (lookup V a) eqn:E; [|easy].
+destruct (extend _) as [V'' new'] eqn:E'.
+eapply IHtry. apply H. eapply intermediate_extend.
+apply E'. all: easy.
+Qed.
 
-Lemma defined_not_new V try new i :
-  Defined V i -> ¬In i (snd (extend_loop V try new)).
-Proof.
-Admitted.
-
-Lemma finished_intermediary V w i :
-  Intermediary V [] -> Defined V i -> w ⊆ gen -> Defined V (apply' w i).
+Lemma intermediate_finished V w i :
+  Intermediate V [] -> Defined V i -> w ⊆ gen -> Defined V (apply' w i).
 Proof.
 intros [_ H]; revert i; simple_ind w.
 apply incl_cons_inv in H1 as []. apply IHw.
@@ -163,15 +242,15 @@ apply H in H0 as []; [easy|apply H0, H1]. easy.
 Qed.
 
 Lemma complete_loop V try i w :
-  w ⊆ gen -> Intermediary V try -> Defined V i ->
+  w ⊆ gen -> Intermediate V try -> Defined V i ->
   Defined (loop V try (length w)) (apply' w i).
 Proof.
 revert V try i; induction w as [|σ w]; [easy|intros; simpl loop].
-destruct (extend_loop _) as [V' new] eqn:E.
-assert(Intermediary V' new). eapply intermediary_extend_loop; [apply E|easy].
+destruct (extend_loop _) as [V' new] eqn:E. assert(Intermediate V' new).
+eapply intermediate_extend_loop. apply E. rewrite app_nil_r; easy.
 eapply defined_extend_loop in H1 as H3; rewrite E in H3; simpl in H3.
-eapply defined_not_new in H1 as H4; rewrite E in H4; simpl in H4.
-destruct new as [|j new]. apply finished_intermediary; easy.
+eapply not_new_extend_loop in H1 as H4; [rewrite E in H4; simpl in H4|easy].
+destruct new as [|j new]. apply intermediate_finished; easy.
 apply incl_cons_inv in H. simpl; apply IHw; try easy.
 destruct H2 as [_ ?]; apply H2 in H3 as []; [easy|].
 apply H3; easy.
@@ -183,8 +262,9 @@ Proof.
 intros H π [w []]; unfold build.
 destruct (short_connecting_word w k) as [w' [? []]].
 assert(w' ⊆ gen) by eauto with datatypes.
-rewrite H1, apply_compose', <-H4.
-eapply defined_loop. apply complete_loop. easy.
+rewrite H1, apply_compose', <-H4. eapply prop_loop_le.
+intros; apply defined_extend_loop; easy.
+apply complete_loop. easy.
 - split. apply Forall_cons. rewrite lookup_insert_eq; easy. auto.
   intros. rewrite lookup_insert in H6.
   destruct (k =? i)%positive eqn:E; [|easy].
